incorportaing docs

ulib/FStar.Pervasives.fst
@@ -18,641 +18,61 @@ module FStar.Pervasives
 
 (* This is a file from the core library, dependencies must be explicit *)
 open Prims
-include FStar.Pervasives.Native
 
-/// This module is implicitly opened in the scope of all other
-/// modules.
-///
-/// It provides several basic definitions in F* that are common to
-/// most programs. Broadly, these include:
-///
-/// - Utility types and functions, like [id], [either], dependent
-///   tuples, etc.
-///
-/// - Utility effect definitions, including [DIV] for divergence,
-///   [EXN] of exceptions, [STATE_h] a template for state, and (the
-///   poorly named) [ALL_h] which combines them all.
-///
-/// - Some utilities to control proofs, e.g., inversion of inductive
-///   type definitions.
-///
-/// - Built-in attributes that can be used to decorate definitions and
-///   trigger various kinds of special treatments for those
-///   definitions.
 
-(** The polymorphic identity function *)
-unfold
-let id (#a: Type) (x: a) : a = x
+/// Implementation of FStar.Pervasives
 
-(** Trivial postconditions for the [PURE] effect *)
-unfold
-let trivial_pure_post (a: Type) : pure_post a = fun _ -> True
+let smt_pat #_ _ = ()
 
-(** Sometimes it is convenient to explicit introduce nullary symbols
-    into the ambient context, so that SMT can appeal to their definitions
-    even when they are no mentioned explicitly in the program, e.g., when
-    needed for triggers.
+let smt_pat_or _ = ()
 
-    Use [intro_ambient t] for that.
-    See, e.g., LowStar.Monotonic.Buffer.fst and its usage there for loc_none *)
-abstract
-let ambient (#a: Type) (x: a) = True
+let ambient #_ _ = True
 
-(** cf. [ambient], above *)
-abstract
-let intro_ambient (#a: Type) (x: a) : squash (ambient x) = ()
+let intro_ambient #_ _ = ()
 
-/// The [DIV] effect for divergent computations
+let inversion _ = True
 
-(** The effect of divergence: from a specificational perspective it is
-    identical to PURE, however the specs are given a partial
-    correctness interpretation. Computations with the [DIV] effect may
-    not terminate. *)
-new_effect DIV = PURE
+let allow_inversion _ = ()
 
-(** [PURE] computations can be silently promoted for use in a [DIV] context *)
-sub_effect PURE ~> DIV { lift_wp = purewp_id }
+let invertOption _ = ()
 
-(** [Div] is the Hoare-style counterpart of the wp-indexed [DIV] *)
-effect Div (a: Type) (pre: pure_pre) (post: pure_post' a pre) =
-  DIV a (fun (p: pure_post a) -> pre /\ (forall a. post a ==> p a))
+let ignore #_ _ = ()
 
-(** [Dv] is the instance of [DIV] with trivial pre- and postconditions *)
-effect Dv (a: Type) = DIV a (fun (p: pure_post a) -> (forall (x: a). p x))
+let rec false_elim #_ _ = false_elim ()
 
-(** We use the [EXT] effect to underspecify external system calls
-    as being impure but having no observable effect on the state *)
-effect EXT (a: Type) = Dv a
+let inline_let = ()
 
-/// The [STATE_h] effect template for stateful computations, generic
-/// in the type of the state.
-///
-/// Note, [STATE_h] is itself not a computation type in F*, since it
-/// is parameterized by the type of heap. However, instantiations of
-/// [STATE_h] with specific types of the heap are computation
-/// types. See, e.g., [FStar.ST] for such instantiations.
-///
-/// Weakest preconditions for stateful computations transform
-/// [st_post_h] postconditions to [st_pre_h] preconditions. Both are
-/// parametric in the type of the state, here denoted by the
-/// [heap:Type] variable.
+let rename_let _ = ()
 
-(** Preconditions are predicates on the [heap] *)
-let st_pre_h (heap: Type) = heap -> GTot Type0
+let plugin _ = ()
 
-(** Postconditions relate [a]-typed results to the final [heap], here
-    refined by some pure proposition [pre], typically instantiated to
-    the precondition applied to the initial [heap] *)
-let st_post_h' (heap a pre: Type) = a -> _: heap{pre} -> GTot Type0
+let tcnorm = ()
 
-(** Postconditions without refinements *)
-let st_post_h (heap a: Type) = st_post_h' heap a True
+let must_erase_for_extraction = ()
 
-(** The type of the main WP-transformer for stateful comptuations *)
-let st_wp_h (heap a: Type) = st_post_h heap a -> Tot (st_pre_h heap)
+let dm4f_bind_range = ()
 
-(** Returning a value does not transform the state *)
-unfold
-let st_return (heap a: Type) (x: a) (p: st_post_h heap a) = p x
+let expect_failure _ = ()
 
-(** Sequential composition of stateful WPs *)
-unfold
-let st_bind_wp
-      (heap: Type)
-      (r1: range)
-      (a b: Type)
-      (wp1: st_wp_h heap a)
-      (wp2: (a -> GTot (st_wp_h heap b)))
-      (p: st_post_h heap b)
-      (h0: heap)
-     = wp1 (fun a h1 -> wp2 a p h1) h0
+let expect_lax_failure _ = ()
 
-(** Branching for stateful WPs *)
-unfold
-let st_if_then_else
-      (heap a p: Type)
-      (wp_then wp_else: st_wp_h heap a)
-      (post: st_post_h heap a)
-      (h0: heap)
-     = l_ITE p (wp_then post h0) (wp_else post h0)
+let tcdecltime = ()
 
-(** As with [PURE] the [ite_wp] combinator names the postcondition as
-    [k] to avoid duplicating it. *)
-unfold
-let st_ite_wp (heap a: Type) (wp: st_wp_h heap a) (post: st_post_h heap a) (h0: heap) =
-  forall (k: st_post_h heap a).
-    (forall (x: a) (h: heap). {:pattern (guard_free (k x h))} post x h ==> k x h) ==> wp k h0
+let assume_strictly_positive = ()
 
-(** Subsumption for stateful WPs *)
-unfold
-let st_stronger (heap a: Type) (wp1 wp2: st_wp_h heap a) =
-  (forall (p: st_post_h heap a) (h: heap). wp1 p h ==> wp2 p h)
+let unifier_hint_injective = ()
 
-(** Closing the scope of a binder within a stateful WP *)
-unfold
-let st_close_wp (heap a b: Type) (wp: (b -> GTot (st_wp_h heap a))) (p: st_post_h heap a) (h: heap) =
-  (forall (b: b). wp b p h)
+let strict_on_arguments _ = ()
 
-(** Applying a stateful WP to a trivial postcondition *)
-unfold
-let st_trivial (heap a: Type) (wp: st_wp_h heap a) = (forall h0. wp (fun r h1 -> True) h0)
+let resolve_implicits = ()
 
-(** Introducing a new effect template [STATE_h] *)
-new_effect {
-  STATE_h (heap: Type) : result: Type -> wp: st_wp_h heap result -> Effect
-  with
-    return_wp = st_return heap
-  ; bind_wp = st_bind_wp heap
-  ; if_then_else = st_if_then_else heap
-  ; ite_wp = st_ite_wp heap
-  ; stronger = st_stronger heap
-  ; close_wp = st_close_wp heap
-  ; trivial = st_trivial heap
-}
+let erasable = ()
 
-/// The [EXN] effect for computations that may raise exceptions or
-/// fatal errors
-///
-/// Weakest preconditions for stateful computations transform
-/// [ex_post] postconditions (predicates on [result]s) to [ex_pre]
-/// precondition propositions.
+let normalize_term #_ x = x
 
-(** Normal results are represented using [V x].
-    Handleable exceptions are represented [E e].
-    Fatal errors are [Err msg]. *)
+let normalize a = a
+
 noeq
-type result (a: Type) =
-  | V : v: a -> result a
-  | E : e: exn -> result a
-  | Err : msg: string -> result a
-
-(** Exceptional preconditions are just propositions *)
-let ex_pre = Type0
-
-(** Postconditions on results refined by a precondition *)
-let ex_post' (a pre: Type) = _: result a {pre} -> GTot Type0
-
-(** Postconditions on results *)
-let ex_post (a: Type) = ex_post' a True
-
-(** Exceptions WP-predicate transformers *)
-let ex_wp (a: Type) = ex_post a -> GTot ex_pre
-
-(** Returning a value [x] normally promotes it to the [V x] result *)
-unfold
-let ex_return (a: Type) (x: a) (p: ex_post a) : GTot Type0 = p (V x)
-
-(** Sequential composition of exception-raising code requires case analysing
-    the result of the first computation before "running" the second one *)
-unfold
-let ex_bind_wp (r1: range) (a b: Type) (wp1: ex_wp a) (wp2: (a -> GTot (ex_wp b))) (p: ex_post b)
-    : GTot Type0 =
-  forall (k: ex_post b).
-    (forall (rb: result b). {:pattern (guard_free (k rb))} p rb ==> k rb) ==>
-    (wp1 (function
-          | V ra1 -> wp2 ra1 k
-          | E e -> k (E e)
-          | Err m -> k (Err m)))
-
-(** As for other effects, branching in [ex_wp] appears in two forms.
-    First, a simple case analysis on [p] *)
-unfold
-let ex_if_then_else (a p: Type) (wp_then wp_else: ex_wp a) (post: ex_post a) =
-  l_ITE p (wp_then post) (wp_else post)
-
-(** Naming continuations for use with branching *)
-unfold
-let ex_ite_wp (a: Type) (wp: ex_wp a) (post: ex_post a) =
-  forall (k: ex_post a).
-    (forall (rb: result a). {:pattern (guard_free (k rb))} post rb ==> k rb) ==> wp k
-
-(** Subsumption for exceptional WPs *)
-unfold
-let ex_stronger (a: Type) (wp1 wp2: ex_wp a) = (forall (p: ex_post a). wp1 p ==> wp2 p)
-
-(** Closing the scope of a binder for exceptional WPs *)
-unfold
-let ex_close_wp (a b: Type) (wp: (b -> GTot (ex_wp a))) (p: ex_post a) = (forall (b: b). wp b p)
-
-(** Applying a computation with a trivial poscondition *)
-unfold
-let ex_trivial (a: Type) (wp: ex_wp a) = wp (fun r -> True)
-
-(** Introduce a new effect for [EXN] *)
-new_effect {
-  EXN : result: Type -> wp: ex_wp result -> Effect
-  with
-    return_wp = ex_return
-  ; bind_wp = ex_bind_wp
-  ; if_then_else = ex_if_then_else
-  ; ite_wp = ex_ite_wp
-  ; stronger = ex_stronger
-  ; close_wp = ex_close_wp
-  ; trivial = ex_trivial
-}
-
-(** A Hoare-style abbreviation for EXN *)
-effect Exn (a: Type) (pre: ex_pre) (post: ex_post' a pre) =
-  EXN a (fun (p: ex_post a) -> pre /\ (forall (r: result a). post r ==> p r))
-
-(** We include divergence in exceptions.
-
-    NOTE: BE WARNED, CODE IN THE [EXN] EFFECT IS ONLY CHECKED FOR
-    PARTIAL CORRECTNESS *)
-unfold
-let lift_div_exn (a: Type) (wp: pure_wp a) (p: ex_post a) = wp (fun a -> p (V a))
-sub_effect DIV ~> EXN { lift_wp = lift_div_exn }
-
-(** A variant of [Exn] with trivial pre- and postconditions *)
-effect Ex (a: Type) = Exn a True (fun v -> True)
-
-/// The [ALL_h] effect template for computations that may diverge,
-/// raise exceptions or fatal errors, and uses a generic state.
-///
-/// Note, this effect is poorly named, particularly as F* has since
-/// gained many more user-defined effect. We no longer have an effect
-/// that includes all others.
-///
-/// We might rename this in the future to something like [StExnDiv_h].
-///
-/// We layer state on top of exceptions, meaning that raising an
-/// exception does not discard the state.
-///
-/// As with [STATE_h], [ALL_h] is not a computation type, though its
-/// instantiation with a specific type of [heap] (in FStar.All) is.
-
-(** [all_pre_h] is a predicate on the initial state *)
-let all_pre_h (h: Type) = h -> GTot Type0
-
-(** Postconditions relate [result]s to final [heap]s refined by a precondition *)
-let all_post_h' (h a pre: Type) = result a -> _: h{pre} -> GTot Type0
-
-(** A variant of [all_post_h'] without the precondition refinement *)
-let all_post_h (h a: Type) = all_post_h' h a True
-
-(** WP predicate transformers for the [All_h] effect template *)
-let all_wp_h (h a: Type) = all_post_h h a -> Tot (all_pre_h h)
-
-(** Returning a value [x] normally promotes it to the [V x] result
-    without touching the [heap] *)
-unfold
-let all_return (heap a: Type) (x: a) (p: all_post_h heap a) = p (V x)
-
-(** Sequential composition for [ALL_h] is like [EXN]: case analysis of
-    the exceptional result before "running" the continuation *)
-unfold
-let all_bind_wp
-      (heap: Type)
-      (r1: range)
-      (a b: Type)
-      (wp1: all_wp_h heap a)
-      (wp2: (a -> GTot (all_wp_h heap b)))
-      (p: all_post_h heap b)
-      (h0: heap)
-    : GTot Type0 =
-  wp1 (fun ra h1 ->
-        (match ra with
-          | V v -> wp2 v p h1
-          | E e -> p (E e) h1
-          | Err msg -> p (Err msg) h1))
-    h0
-
-(** Case analysis in [ALL_h] *)
-unfold
-let all_if_then_else
-      (heap a p: Type)
-      (wp_then wp_else: all_wp_h heap a)
-      (post: all_post_h heap a)
-      (h0: heap)
-     = l_ITE p (wp_then post h0) (wp_else post h0)
-
-(** Naming postcondition for better sharing in [ALL_h] *)
-unfold
-let all_ite_wp (heap a: Type) (wp: all_wp_h heap a) (post: all_post_h heap a) (h0: heap) =
-  forall (k: all_post_h heap a).
-    (forall (x: result a) (h: heap). {:pattern (guard_free (k x h))} post x h ==> k x h) ==> wp k h0
-
-(** Subsumption in [ALL_h] *)
-unfold
-let all_stronger (heap a: Type) (wp1 wp2: all_wp_h heap a) =
-  (forall (p: all_post_h heap a) (h: heap). wp1 p h ==> wp2 p h)
-
-(** Closing a binder in the scope of an [ALL_h] wp *)
-unfold
-let all_close_wp
-      (heap a b: Type)
-      (wp: (b -> GTot (all_wp_h heap a)))
-      (p: all_post_h heap a)
-      (h: heap)
-     = (forall (b: b). wp b p h)
-
-(** Applying an [ALL_h] wp to a trivial postcondition *)
-unfold
-let all_trivial (heap a: Type) (wp: all_wp_h heap a) = (forall (h0: heap). wp (fun r h1 -> True) h0)
-
-(** Introducing the [ALL_h] effect template *)
-new_effect {
-  ALL_h (heap: Type) : a: Type -> wp: all_wp_h heap a -> Effect
-  with
-    return_wp = all_return heap
-  ; bind_wp = all_bind_wp heap
-  ; if_then_else = all_if_then_else heap
-  ; ite_wp = all_ite_wp heap
-  ; stronger = all_stronger heap
-  ; close_wp = all_close_wp heap
-  ; trivial = all_trivial heap
-}
-
-(**
- Controlling inversions of inductive type
-
- Given a value of an inductive type [v:t], where [t = A | B], the SMT
- solver can only prove that [v=A \/ v=B] by _inverting_ [t]. This
- inversion is controlled by the [ifuel] setting, which usually limits
- the recursion depth of the number of such inversions that the solver
- can perform.
-
- The [inversion] predicate below is a way to circumvent the
- [ifuel]-based restrictions on inversion depth. In particular, if the
- [inversion t] is available in the SMT solver's context, it is free to
- invert [t] infinitely, regardless of the [ifuel] setting.
-
- Be careful using this, since it explicitly subverts the [ifuel]
- setting. If used unwisely, this can lead to very poor SMT solver
- performance.  *)
-let inversion (a: Type) = True
-
-(** To introduce [inversion t] in the SMT solver's context, call
-    [allow_inverson t]. *)
-let allow_inversion (a: Type) : Pure unit (requires True) (ensures (fun x -> inversion a)) = ()
-
-(** Since the [option] type is so common, we always allow inverting
-    options, regardless of [ifuel] *)
-let invertOption (a: Type)
-    : Lemma (requires True) (ensures (forall (x: option a). None? x \/ Some? x)) [SMTPat (option a)] =
-  allow_inversion (option a)
-
-(** Values of type [a] or type [b] *)
-type either a b =
-  | Inl : v: a -> either a b
-  | Inr : v: b -> either a b
-
-(** Projections for the components of a dependent pair *)
-val dfst: #a: Type -> #b: (a -> GTot Type) -> dtuple2 a b -> Tot a
-let dfst #a #b t = Mkdtuple2?._1 t
-
-val dsnd (#a: Type) (#b: (a -> GTot Type)) (t: dtuple2 a b) : Tot (b (Mkdtuple2?._1 t))
-let dsnd #a #b t = Mkdtuple2?._2 t
-
-(** Dependent triples, with sugar [x:a & y:b x & c x y] *)
-unopteq
-type dtuple3 (a: Type) (b: (a -> GTot Type)) (c: (x: a -> b x -> GTot Type)) =
-  | Mkdtuple3 : _1: a -> _2: b _1 -> _3: c _1 _2 -> dtuple3 a b c
-
-(** Dependent quadruples, with sugar [x:a & y:b x & z:c x y & d x y z] *)
-unopteq
-type dtuple4
-  (a: Type) (b: (x: a -> GTot Type)) (c: (x: a -> b x -> GTot Type))
-  (d: (x: a -> y: b x -> z: c x y -> GTot Type))
-  = | Mkdtuple4 : _1: a -> _2: b _1 -> _3: c _1 _2 -> _4: d _1 _2 _3 -> dtuple4 a b c d
-
-(** Explicitly discarding a value *)
-let ignore (#a: Type) (x: a) : Tot unit = ()
-
-(** In a context where [false] is provable, you can prove that any
-    type [a] is inhabited.
-
-    There are many proofs of this fact in F*. Here, we build an
-    infinitely looping function, since the termination check succeeds
-    in a [False] context. *)
-irreducible
-let rec false_elim (#a: Type) (u: unit{False}) : Tot a = false_elim ()
-
-/// Attributes:
-///
-/// An attribute is any F* term.
-///
-/// Attributes are desugared and checked for being well-scoped. But,
-/// they are not type-checked.
-///
-/// It is associated with a definition using the [[@attribute]]
-/// notation, just preceding the definition.
-
-(** We collect several internal ocaml attributes into a single
-    inductive type.
-
-    This may be unnecessary. In the future, we are likely to flatten
-    this definition into several definitions of abstract top-level
-    names.
-
-    An example:
-
-     {[
-        [@ CInline ] let f x = UInt32.(x +%^ 1)
-      ]}
-
-    is extracted to C by KReMLin to a C definition tagged with the
-    [inline] qualifier. *)
-type __internal_ocaml_attributes =
-  | PpxDerivingShow
-  | PpxDerivingShowConstant of string (* Generate [@@ deriving show ] on the resulting OCaml type *)
-  | PpxDerivingYoJson (* Similar, but for constant printers. *)
-  | CInline (* Generate [@@ deriving yojson ] on the resulting OCaml type *)
-  (* KreMLin-only: generates a C "inline" attribute on the resulting
-     * function declaration. *)
-  | Substitute
-  (* KreMLin-only: forces KreMLin to inline the function at call-site; this is
-     * deprecated and the recommended way is now to use F*'s
-     * [inline_for_extraction], which now also works for stateful functions. *)
-  | Gc
-  (* KreMLin-only: instructs KreMLin to heap-allocate any value of this
-     * data-type; this requires running with a conservative GC as the
-     * allocations are not freed. *)
-  | Comment of string
-  (* KreMLin-only: attach a comment to the declaration. Note that using F*-doc
-     * syntax automatically fills in this attribute. *)
-  | CPrologue of string
-  (* KreMLin-only: verbatim C code to be prepended to the declaration.
-     * Multiple attributes are valid and accumulate, separated by newlines. *)
-  | CEpilogue of string
-  | CConst of string (* Ibid. *)
-  (* KreMLin-only: indicates that the parameter with that name is to be marked
-     * as C const.  This will be checked by the C compiler, not by KreMLin or F*.
-     *
-     * This is deprecated and doesn't work as intended. Use
-     * LowStar.ConstBuffer.fst instead! *)
-  | CCConv of string
-  | CAbstractStruct (* A calling convention for C, one of stdcall, cdecl, fastcall *)
-  (* KreMLin-only: for types that compile to struct types (records and
-     * inductives), indicate that the header file should only contain a forward
-     * declaration, which in turn forces the client to only ever use this type
-     * through a pointer. *)
-  | CIfDef
-  | CMacro (* KreMLin-only: on a given `val foo`, compile if foo with #ifdef. *)
-(* KreMLin-only: for a top-level `let v = e`, compile as a macro *)
-
-(** The [inline_let] attribute on a local let-binding, instructs the
-    extraction pipeline to inline the definition. This may be both to
-    avoid generating unnecessary intermediate variables, and also to
-    enable further partial evaluation. Note, use this with care, since
-    inlining all lets can lead to an exponential blowup in code
-    size. *)
-irreducible
-let inline_let:unit = ()
-
-(** The [rename_let] attribute support a form of metaprogramming for
-    the names of let-bound variables used in extracted code.
-
-    This is useful, particularly in conjunction with partial
-    evaluation, to ensure that names reflect their usage context.
-
-    See examples/micro-benchmarks/Renaming*.fst *)
-irreducible
-let rename_let (new_name: string) : unit = ()
-
-(** The [plugin] attribute is used in conjunction with native
-    compilation of F* components, accelerating their reduction
-    relative to the default strategy of just interpreting them.
-
-    See examples/native_tactics for several examples. *)
-irreducible
-let plugin (x: int) : unit = ()
-
-(** An attribute to mark things that the typechecker should *first*
-    elaborate and typecheck, but unfold before verification. *)
-irreducible
-let tcnorm:unit = ()
-
-(** We erase all ghost functions and unit-returning pure functions to
-    [()] at extraction. This creates a small issue with abstract
-    types. Consider a module that defines an abstract type [t] whose
-    (internal) definition is [unit] and also defines [f: int -> t]. [f]
-    would be erased to be just [()] inside the module, while the
-    client calls to [f] would not, since [t] is abstract. To get
-    around this, when extracting interfaces, if we encounter an
-    abstract type, we tag it with this attribute, so that
-    extraction can treat it specially.
-
-    Note, since the use of cross-module inlining (the [--cmi] option),
-    this attribute is no longer necessary. We retain it for legacy,
-    but will remove it in the future. *)
-irreducible
-let must_erase_for_extraction:unit = ()
-
-(** This attribute is used with the Dijkstra Monads for Free
-    construction to track position information in generated VCs *)
-let dm4f_bind_range:unit = ()
-
-(** When attached a top-level definition, the typechecker will succeed
-    if and only if checking the definition results in an error. The
-    error number list is actually OPTIONAL. If present, it will be
-    checked that the definition raises exactly those errors in the
-    specified multiplicity, but order does not matter. *)
-irreducible
-let expect_failure (errs: list int) : unit = ()
-
-(** When --lax is present, with the previous attribute since some
-  definitions only fail when verification is turned on. With this
-  attribute, one can ensure that a definition fails while lax-checking
-  too. Same semantics as above, but lax mode will be turned on for the
-  definition.  *)
-irreducible
-let expect_lax_failure (errs: list int) : unit = ()
-
-(** Print the time it took to typecheck a top-level definition *)
-irreducible
-let tcdecltime:unit = ()
-
-(** **THIS ATTRIBUTE IS AN ESCAPE HATCH AND CAN BREAK SOUNDNESS**
-
-    **USE WITH CARE**
-
-    The positivity check for inductive types stops at abstraction
-    boundaries. This results in spurious errors about positivity,
-    e.g., when defining types like `type t = ref (option t)` By adding
-    this attribute to a declaration of a top-level name positivity
-    checks on applications of that name are admitted.  See, for
-    instance, FStar.Monotonic.Heap.mref We plan to decorate binders of
-    abstract types with polarities to allow us to check positivity
-    across abstraction boundaries and will eventually remove this
-    attribute.  *)
-irreducible
-let assume_strictly_positive:unit = ()
-
-(** This attribute is to be used as a hint for the unifier.  A
-    function-typed symbol `t` marked with this attribute will be treated
-    as being injective in all its arguments by the unifier.  That is,
-    given a problem `t a1..an =?= t b1..bn` the unifier will solve it by
-    proving `ai =?= bi` for all `i`, without trying to unfold the
-    definition of `t`. *)
-irreducible
-let unifier_hint_injective:unit = ()
-
-(**
- This attribute is used to control the evaluation order
- and unfolding strategy for certain definitions.
-
-  In particular, given
-     {[
-        [@(strict_on_arguments [1;2])]
-        let f x0 (x1:list x0) (x1:option x0) = e
-     ]}
-
- An application [f e0 e1 e2] is reduced by the normalizer by:
-
-     1. evaluating [e0 ~>* v0, e1 ~>* v1, e2 ~>* v2]
-
-     2 a.
-        If, according to the positional arguments [1;2],
-        if v1 and v2 have constant head symbols
-              (e.g., v1 = Cons _ _ _, and v2 = None _)
-       then [f] is unfolded to [e] and reduced as
-         {[e[v0/x0][v1/x1][v2/x2]]}
-
-     2 b.
-
-      Otherwise, [f] is not unfolded and the term is [f e0 e1 e2]
-      reduces to [f v0 v1 v2]. *)
-irreducible
-let strict_on_arguments (x: list int) : unit = ()
-
-(**
- * An attribute to tag a tactic designated to solve any
- * unsolved implicit arguments remaining at the end of type inference.
- **)
-irreducible
-let resolve_implicits : unit = ()
-
-(** This attribute can be added to an inductive type definition,
-    indicating that it should be erased on extraction to `unit`.
-
-    However, any pattern matching on the inductive type results
-    in a `Ghost` effect, ensuring that computationally relevant
-    code cannot rely on the values of the erasable type.
-
-    See examples/micro-benchmarks/Erasable.fst, for examples.  Also
-    see https://github.com/FStarLang/FStar/issues/1844 *)
-irreducible
-let erasable:unit = ()
-
-///  Controlling normalization
-
-(** In any invocation of the F* normalizer, every occurrence of
-    [normalize_term e] is reduced to the full normal for of [e]. *)
-abstract
-let normalize_term (#a: Type) (x: a) : a = x
-
-(** In any invocation of the F* normalizer, every occurrence of
-    [normalize e] is reduced to the full normal for of [e]. *)
-abstract
-let normalize (a: Type0) : Type0 = a
-
-(** Value of [norm_step] are used to enable specific normalization
-    steps, controlling how the normalizer reduces terms.
-
-    We wrap the inductive type with helpers (below), so we don't
-    expose the actual inductive *)
-abstract noeq
 type norm_step =
   | Simpl // Logical simplification, e.g., [P /\ True ~> P]
   | Weak // Weak reduction: Do not reduce under binders
@@ -670,126 +90,40 @@ type norm_step =
   | UnfoldFully : list string -> norm_step
   | UnfoldAttr : list string -> norm_step // Unfold definitions marked with the given attributes
 
-(** Logical simplification, e.g., [P /\ True ~> P] *)
-abstract
-let simplify:norm_step = Simpl
+let simplify = Simpl
 
-(** Weak reduction: Do not reduce under binders *)
-abstract
-let weak:norm_step = Weak
+let weak = Weak
 
-(** Head normal form *)
-abstract
-let hnf:norm_step = HNF
+let hnf = HNF
 
-(** Reduce primitive operators, e.g., [1 + 1 ~> 2] *)
-abstract
-let primops:norm_step = Primops
+let primops = Primops
 
-(** Unfold all non-recursive definitions *)
-abstract
-let delta:norm_step = Delta
+let delta = Delta
 
-(** Unroll recursive calls *)
-abstract
-let zeta:norm_step = Zeta
+let zeta = Zeta
 
-(** Reduce case analysis (i.e., match) *)
-abstract
-let iota:norm_step = Iota
+let iota = Iota
 
-(** Use normalization-by-evaluation, instead of interpretation (experimental) *)
-abstract
-let nbe:norm_step = NBE
+let nbe = NBE
 
-(** Reify effectful definitions into their representations *)
-abstract
-let reify_:norm_step = Reify
+let reify_ = Reify
 
-(** Unlike [delta], unfold definitions for only the names in the given
-    list. Each string is a fully qualified name like [A.M.f] *)
-abstract
-let delta_only (s: list string) : norm_step = UnfoldOnly s
+let delta_only s = UnfoldOnly s
 
-(** Unfold definitions for only the names in the given list, but
-    unfold each definition encountered after unfolding as well.
+let delta_fully s = UnfoldFully s
 
-    For example, given
+let delta_attr s = UnfoldAttr s
 
-      {[
-        let f0 = 0
-        let f1 = f0 + 1
-      ]}
+let norm _ #_ x = x
 
-    [norm [delta_only [`%f1]] f1] will reduce to [f0 + 1].
-    [norm [delta_fully [`%f1]] f1] will reduce to [0 + 1].
+let assert_norm _ = ()
 
-    Each string is a fully qualified name like [A.M.f], typically
-    constructed using a quotation, as in the example above. *)
-abstract
-let delta_fully (s: list string) : norm_step = UnfoldFully s
+let normalize_term_spec #_ _ = ()
 
-(** Rather than mention a symbol to unfold by name, it can be
-    convenient to tag a collection of related symbols with a common
-    attribute and then to ask the normalizer to reduce them all.
+let normalize_spec _ = ()
 
-    For example, given:
+let norm_spec _ #_ _ = ()
 
-      {[
-        irreducible let my_attr = ()
+let singleton #_ x = x
 
-        [@my_attr]
-        let f0 = 0
-
-        [@my_attr]
-        let f1 = f0 + 1
-      ]}
-
-   {[norm [delta_attr [`%my_attr]] f1]}
-   
-   will reduce to [0 + 1].
-
-  *)
-abstract
-let delta_attr (s: list string) : norm_step = UnfoldAttr s
-
-(** [norm s e] requests normalization of [e] with the reduction steps
-    [s]. *)
-abstract
-let norm (s: list norm_step) (#a: Type) (x: a) : a = x
-
-(** [assert_norm p] reduces [p] as much as possible and then asks the
-    SMT solver to prove the reduct, concluding [p] *)
-abstract
-val assert_norm (p: Type) : Pure unit (requires (normalize p)) (ensures (fun _ -> p))
-let assert_norm p = ()
-
-(** Sometimes it is convenient to introduce an equation between a term
-    and its normal form in the context. *)
-let normalize_term_spec (#a: Type) (x: a) : Lemma (normalize_term #a x == x) = ()
-
-(** Like [normalize_term_spec], but specialized to [Type0] *)
-let normalize_spec (a: Type0) : Lemma (normalize a == a) = ()
-
-(** Like [normalize_term_spec], but with specific normalization steps *)
-let norm_spec (s: list norm_step) (#a: Type) (x: a) : Lemma (norm s #a x == x) = ()
-
-(** Use the following to expose an ["opaque_to_smt"] definition to the
-    solver as: [reveal_opaque (`%defn) defn] *)
-let reveal_opaque (s: string) = norm_spec [delta_only [s]]
-
-(** Pure and ghost inner let bindings are now always inlined during
-    the wp computation, if: the return type is not unit and the head
-    symbol is not marked irreducible.
-
-    To circumvent this behavior, singleton can be used.
-    See the example usage in ulib/FStar.Algebra.Monoid.fst. *)
-irreducible
-let singleton (#a: Type) (x: a) : (y: a{y == x}) = x
-
-(** [with_type t e] is just an identity function, but it receives
-    special treatment in the SMT encoding, where in addition to being
-    an identity function, we have an SMT axiom:
-    [forall t e.{:pattern (with_type t e)} has_type (with_type t e) t] *)
-let with_type (#t: Type) (e: t) = e
-
+let with_type #_ e = e
