ulib/FStar.Pervasives.fsti
@@ -13,433 +13,611 @@
    See the License for the specific language governing permissions and
    limitations under the License.
 *)
+
 module FStar.Pervasives
 
 (* This is a file from the core library, dependencies must be explicit *)
 open Prims
 include FStar.Pervasives.Native
 
-val pattern : Type0
+/// This module is implicitly opened in the scope of all other
+/// modules.
+///
+/// It provides several basic definitions in F* that are common to
+/// most programs. Broadly, these include:
+///
+/// - Utility types and functions, like [id], [either], dependent
+///   tuples, etc.
+///
+/// - Utility effect definitions, including [DIV] for divergence,
+///   [EXN] of exceptions, [STATE_h] a template for state, and (the
+///   poorly named) [ALL_h] which combines them all.
+///
+/// - Some utilities to control proofs, e.g., inversion of inductive
+///   type definitions.
+///
+/// - Built-in attributes that can be used to decorate definitions and
+///   trigger various kinds of special treatments for those
+///   definitions.
 
-// SMTPat and SMTPatOr desugar to these two
-val smt_pat (#a:Type) (x:a) : Tot pattern
+(** The concrete syntax [SMTPat] desugars to [smt_pat] *)
+val smt_pat (#a: Type) (x: a) : pattern
 
-val smt_pat_or (x:list (list pattern)) : Tot pattern
+(** The concrete syntax [SMTPatOr] desugars to [smt_pat_or]. This is
+    used to represent a disjunction of conjunctions of patterns.
 
-// Can be used to mark a query for a separate SMT invocation
-val spinoff (p:Type0) : Type0
+    Note, the typing discipline and syntax of patterns is laxer than
+    it should be. Patterns like [SMTPatOr [SMTPatOr [...]]] are
+    expressible, but unsupported by F*
 
-// Logically equivalent to assert, but spins off separate query
-val assert_spinoff : (p:Type) -> Pure unit (requires (spinoff (squash p))) (ensures (fun x -> p))
-
-
-(*
-   Lemma is desugared specially. The valid forms are:
-
-     Lemma (ensures post)
-     Lemma post [SMTPat ...]
-     Lemma (ensures post) [SMTPat ...]
-     Lemma (ensures post) (decreases d)
-     Lemma (ensures post) (decreases d) [SMTPat ...]
-     Lemma (requires pre) (ensures post) (decreases d)
-     Lemma (requires pre) (ensures post) [SMTPat ...]
-     Lemma (requires pre) (ensures post) (decreases d) [SMTPat ...]
-
-   and
-
-     Lemma post    (== Lemma (ensures post))
-
-   the squash argument on the postcondition allows to assume the
-   precondition for the *well-formedness* of the postcondition.
-   C.f. #57.
+    TODO: We should tighten this up, perhaps just reusing the
+    attribute mechanism for patterns.
 *)
-effect Lemma (a:Type) (pre:Type) (post:squash pre -> Type) (pats:list pattern) =
-       Pure a pre (fun r -> post ())
+val smt_pat_or (x: list (list pattern)) : pattern
 
-
+(** The polymorphic identity function *)
 unfold
-let id (#a:Type) (x:a) : a = x
+let id (#a: Type) (x: a) : a = x
 
+(** Trivial postconditions for the [PURE] effect *)
 unfold
-let trivial_pure_post (a:Type) : pure_post a = fun _ -> True
+let trivial_pure_post (a: Type) : pure_post a = fun _ -> True
 
-(* Sometimes it is convenient to explicit introduce nullary symbols
- * into the ambient context, so that SMT can appeal to their definitions
- * even when they are no mentioned explicitly in the program, e.g., when
- * needed for triggers.
- * Use `intro_ambient t` for that.
- * See, e.g., LowStar.Monotonic.Buffer.fst and its usage there for loc_none
- *)
-val ambient (#a:Type) (x:a) : Type0
-val intro_ambient (#a:Type) (x:a) : Tot (squash (ambient x))
+(** Sometimes it is convenient to explicit introduce nullary symbols
+    into the ambient context, so that SMT can appeal to their definitions
+    even when they are no mentioned explicitly in the program, e.g., when
+    needed for triggers.
 
+    Use [intro_ambient t] for that.
+    See, e.g., LowStar.Monotonic.Buffer.fst and its usage there for loc_none *)
+val ambient (#a: Type) (x: a) : Type0
+
+(** cf. [ambient], above *)
+val intro_ambient (#a: Type) (x: a) : Tot (squash (ambient x))
+
+
+/// The [DIV] effect for divergent computations
+
+(** The effect of divergence: from a specificational perspective it is
+    identical to PURE, however the specs are given a partial
+    correctness interpretation. Computations with the [DIV] effect may
+    not terminate. *)
 new_effect DIV = PURE
-sub_effect PURE ~> DIV  = purewp_id
 
-effect Div (a:Type) (pre:pure_pre) (post:pure_post' a pre) =
-       DIV a (fun (p:pure_post a) -> pre /\ (forall a. post a ==> p a))
+(** [PURE] computations can be silently promoted for use in a [DIV] context *)
+sub_effect PURE ~> DIV { lift_wp = purewp_id }
 
-effect Dv (a:Type) =
-     DIV a (fun (p:pure_post a) -> (forall (x:a). p x))
+(** [Div] is the Hoare-style counterpart of the wp-indexed [DIV] *)
+effect Div (a: Type) (pre: pure_pre) (post: pure_post' a pre) =
+  DIV a (fun (p: pure_post a) -> pre /\ (forall a. post a ==> p a))
 
-(* We use the EXT effect to underspecify external system calls
-   as being impure but having no observable effect on the state *)
-effect EXT (a:Type) = Dv a
+(** [Dv] is the instance of [DIV] with trivial pre- and postconditions *)
+effect Dv (a: Type) = DIV a (fun (p: pure_post a) -> (forall (x: a). p x))
 
-let st_pre_h   (heap:Type) = heap -> GTot Type0
-let st_post_h' (heap:Type) (a:Type) (pre:Type) = a -> (_:heap{pre}) -> GTot Type0
-let st_post_h  (heap:Type) (a:Type) = st_post_h' heap a True
-let st_wp_h    (heap:Type) (a:Type) = st_post_h heap a -> Tot (st_pre_h heap)
+(** We use the [EXT] effect to underspecify external system calls
+    as being impure but having no observable effect on the state *)
+effect EXT (a: Type) = Dv a
 
-unfold let st_return        (heap:Type) (a:Type)
-                            (x:a) (p:st_post_h heap a) =
-     p x
-unfold let st_bind_wp       (heap:Type)
-			    (r1:range)
-			    (a:Type) (b:Type)
-                            (wp1:st_wp_h heap a)
-                            (wp2:(a -> GTot (st_wp_h heap b)))
-                            (p:st_post_h heap b) (h0:heap) =
-  wp1 (fun a h1 -> wp2 a p h1) h0
-unfold let st_if_then_else  (heap:Type) (a:Type) (p:Type)
-                             (wp_then:st_wp_h heap a) (wp_else:st_wp_h heap a)
-                             (post:st_post_h heap a) (h0:heap) =
-     l_ITE p
-        (wp_then post h0)
-	(wp_else post h0)
-unfold let st_ite_wp        (heap:Type) (a:Type)
-                            (wp:st_wp_h heap a)
-                            (post:st_post_h heap a) (h0:heap) =
-     forall (k:st_post_h heap a).
-	 (forall (x:a) (h:heap).{:pattern (guard_free (k x h))} post x h ==> k x h)
-	 ==> wp k h0
-unfold let st_stronger  (heap:Type) (a:Type) (wp1:st_wp_h heap a)
-                        (wp2:st_wp_h heap a) =
-     (forall (p:st_post_h heap a) (h:heap). wp1 p h ==> wp2 p h)
+/// The [STATE_h] effect template for stateful computations, generic
+/// in the type of the state.
+///
+/// Note, [STATE_h] is itself not a computation type in F*, since it
+/// is parameterized by the type of heap. However, instantiations of
+/// [STATE_h] with specific types of the heap are computation
+/// types. See, e.g., [FStar.ST] for such instantiations.
+///
+/// Weakest preconditions for stateful computations transform
+/// [st_post_h] postconditions to [st_pre_h] preconditions. Both are
+/// parametric in the type of the state, here denoted by the
+/// [heap:Type] variable.
 
-unfold let st_close_wp      (heap:Type) (a:Type) (b:Type)
-                             (wp:(b -> GTot (st_wp_h heap a)))
-                             (p:st_post_h heap a) (h:heap) =
-     (forall (b:b). wp b p h)
-unfold let st_trivial       (heap:Type) (a:Type)
-                             (wp:st_wp_h heap a) =
-     (forall h0. wp (fun r h1 -> True) h0)
+(** Preconditions are predicates on the [heap] *)
+let st_pre_h (heap: Type) = heap -> GTot Type0
 
+(** Postconditions relate [a]-typed results to the final [heap], here
+    refined by some pure proposition [pre], typically instantiated to
+    the precondition applied to the initial [heap] *)
+let st_post_h' (heap a pre: Type) = a -> _: heap{pre} -> GTot Type0
+
+(** Postconditions without refinements *)
+let st_post_h (heap a: Type) = st_post_h' heap a True
+
+(** The type of the main WP-transformer for stateful comptuations *)
+let st_wp_h (heap a: Type) = st_post_h heap a -> Tot (st_pre_h heap)
+
+(** Returning a value does not transform the state *)
+unfold
+let st_return (heap a: Type) (x: a) (p: st_post_h heap a) = p x
+
+(** Sequential composition of stateful WPs *)
+unfold
+let st_bind_wp
+      (heap: Type)
+      (r1: range)
+      (a b: Type)
+      (wp1: st_wp_h heap a)
+      (wp2: (a -> GTot (st_wp_h heap b)))
+      (p: st_post_h heap b)
+      (h0: heap)
+     = wp1 (fun a h1 -> wp2 a p h1) h0
+
+(** Branching for stateful WPs *)
+unfold
+let st_if_then_else
+      (heap a p: Type)
+      (wp_then wp_else: st_wp_h heap a)
+      (post: st_post_h heap a)
+      (h0: heap)
+     = l_ITE p (wp_then post h0) (wp_else post h0)
+
+(** As with [PURE] the [ite_wp] combinator names the postcondition as
+    [k] to avoid duplicating it. *)
+unfold
+let st_ite_wp (heap a: Type) (wp: st_wp_h heap a) (post: st_post_h heap a) (h0: heap) =
+  forall (k: st_post_h heap a).
+    (forall (x: a) (h: heap). {:pattern (guard_free (k x h))} post x h ==> k x h) ==> wp k h0
+
+(** Subsumption for stateful WPs *)
+unfold
+let st_stronger (heap a: Type) (wp1 wp2: st_wp_h heap a) =
+  (forall (p: st_post_h heap a) (h: heap). wp1 p h ==> wp2 p h)
+
+(** Closing the scope of a binder within a stateful WP *)
+unfold
+let st_close_wp (heap a b: Type) (wp: (b -> GTot (st_wp_h heap a))) (p: st_post_h heap a) (h: heap) =
+  (forall (b: b). wp b p h)
+
+(** Applying a stateful WP to a trivial postcondition *)
+unfold
+let st_trivial (heap a: Type) (wp: st_wp_h heap a) = (forall h0. wp (fun r h1 -> True) h0)
+
+(** Introducing a new effect template [STATE_h] *)
 new_effect {
-  STATE_h (heap:Type) : result:Type -> wp:st_wp_h heap result -> Effect
-  with return_wp    = st_return heap
-     ; bind_wp      = st_bind_wp heap
-     ; if_then_else = st_if_then_else heap
-     ; ite_wp       = st_ite_wp heap
-     ; stronger     = st_stronger heap
-     ; close_wp     = st_close_wp heap
-     ; trivial      = st_trivial heap
+  STATE_h (heap: Type) : result: Type -> wp: st_wp_h heap result -> Effect
+  with
+    return_wp = st_return heap
+  ; bind_wp = st_bind_wp heap
+  ; if_then_else = st_if_then_else heap
+  ; ite_wp = st_ite_wp heap
+  ; stronger = st_stronger heap
+  ; close_wp = st_close_wp heap
+  ; trivial = st_trivial heap
 }
 
+/// The [EXN] effect for computations that may raise exceptions or
+/// fatal errors
+///
+/// Weakest preconditions for stateful computations transform
+/// [ex_post] postconditions (predicates on [result]s) to [ex_pre]
+/// precondition propositions.
 
-noeq type result (a:Type) =
-  | V   : v:a -> result a
-  | E   : e:exn -> result a
-  | Err : msg:string -> result a
+(** Normal results are represented using [V x].
+    Handleable exceptions are represented [E e].
+    Fatal errors are [Err msg]. *)
+noeq
+type result (a: Type) =
+  | V : v: a -> result a
+  | E : e: exn -> result a
+  | Err : msg: string -> result a
 
-(* Effect EXCEPTION *)
-let ex_pre  = Type0
-let ex_post' (a:Type) (pre:Type) = (_:result a{pre}) -> GTot Type0
-let ex_post  (a:Type) = ex_post' a True
-let ex_wp    (a:Type) = ex_post a -> GTot ex_pre
-unfold let ex_return   (a:Type) (x:a) (p:ex_post a) : GTot Type0 = p (V x)
-unfold let ex_bind_wp (r1:range) (a:Type) (b:Type)
-		       (wp1:ex_wp a)
-		       (wp2:(a -> GTot (ex_wp b))) (p:ex_post b)
-         : GTot Type0 =
-  forall (k:ex_post b).
-     (forall (rb:result b).{:pattern (guard_free (k rb))} p rb ==> k rb)
-     ==> (wp1 (function
-               | V ra1 -> wp2 ra1 k
-               | E e -> k (E e)
-               | Err m -> k (Err m)))
+(** Exceptional preconditions are just propositions *)
+let ex_pre = Type0
 
-unfold let ex_ite_wp (a:Type) (wp:ex_wp a) (post:ex_post a) =
-  forall (k:ex_post a).
-     (forall (rb:result a).{:pattern (guard_free (k rb))} post rb ==> k rb)
-     ==> wp k
+(** Postconditions on results refined by a precondition *)
+let ex_post' (a pre: Type) = _: result a {pre} -> GTot Type0
 
-unfold let ex_if_then_else (a:Type) (p:Type) (wp_then:ex_wp a) (wp_else:ex_wp a) (post:ex_post a) =
-   l_ITE p
-       (wp_then post)
-       (wp_else post)
-unfold let ex_stronger (a:Type) (wp1:ex_wp a) (wp2:ex_wp a) =
-        (forall (p:ex_post a). wp1 p ==> wp2 p)
+(** Postconditions on results *)
+let ex_post (a: Type) = ex_post' a True
 
-unfold let ex_close_wp (a:Type) (b:Type) (wp:(b -> GTot (ex_wp a))) (p:ex_post a) = (forall (b:b). wp b p)
-unfold let ex_trivial (a:Type) (wp:ex_wp a) = wp (fun r -> True)
+(** Exceptions WP-predicate transformers *)
+let ex_wp (a: Type) = ex_post a -> GTot ex_pre
 
+(** Returning a value [x] normally promotes it to the [V x] result *)
+unfold
+let ex_return (a: Type) (x: a) (p: ex_post a) : GTot Type0 = p (V x)
+
+(** Sequential composition of exception-raising code requires case analysing
+    the result of the first computation before "running" the second one *)
+unfold
+let ex_bind_wp (r1: range) (a b: Type) (wp1: ex_wp a) (wp2: (a -> GTot (ex_wp b))) (p: ex_post b)
+    : GTot Type0 =
+  forall (k: ex_post b).
+    (forall (rb: result b). {:pattern (guard_free (k rb))} p rb ==> k rb) ==>
+    (wp1 (function
+          | V ra1 -> wp2 ra1 k
+          | E e -> k (E e)
+          | Err m -> k (Err m)))
+
+(** As for other effects, branching in [ex_wp] appears in two forms.
+    First, a simple case analysis on [p] *)
+unfold
+let ex_if_then_else (a p: Type) (wp_then wp_else: ex_wp a) (post: ex_post a) =
+  l_ITE p (wp_then post) (wp_else post)
+
+(** Naming continuations for use with branching *)
+unfold
+let ex_ite_wp (a: Type) (wp: ex_wp a) (post: ex_post a) =
+  forall (k: ex_post a).
+    (forall (rb: result a). {:pattern (guard_free (k rb))} post rb ==> k rb) ==> wp k
+
+(** Subsumption for exceptional WPs *)
+unfold
+let ex_stronger (a: Type) (wp1 wp2: ex_wp a) = (forall (p: ex_post a). wp1 p ==> wp2 p)
+
+(** Closing the scope of a binder for exceptional WPs *)
+unfold
+let ex_close_wp (a b: Type) (wp: (b -> GTot (ex_wp a))) (p: ex_post a) = (forall (b: b). wp b p)
+
+(** Applying a computation with a trivial poscondition *)
+unfold
+let ex_trivial (a: Type) (wp: ex_wp a) = wp (fun r -> True)
+
+(** Introduce a new effect for [EXN] *)
 new_effect {
-  EXN : result:Type -> wp:ex_wp result -> Effect
+  EXN : result: Type -> wp: ex_wp result -> Effect
   with
-    return_wp    = ex_return
-  ; bind_wp      = ex_bind_wp
+    return_wp = ex_return
+  ; bind_wp = ex_bind_wp
   ; if_then_else = ex_if_then_else
-  ; ite_wp       = ex_ite_wp
-  ; stronger     = ex_stronger
-  ; close_wp     = ex_close_wp
-  ; trivial      = ex_trivial
+  ; ite_wp = ex_ite_wp
+  ; stronger = ex_stronger
+  ; close_wp = ex_close_wp
+  ; trivial = ex_trivial
 }
-effect Exn (a:Type) (pre:ex_pre) (post:ex_post' a pre) =
-       EXN a (fun (p:ex_post a) -> pre /\ (forall (r:result a). post r ==> p r))
 
-unfold let lift_div_exn (a:Type) (wp:pure_wp a) (p:ex_post a) = wp (fun a -> p (V a))
-sub_effect DIV ~> EXN = lift_div_exn
-effect Ex (a:Type) = Exn a True (fun v -> True)
+(** A Hoare-style abbreviation for EXN *)
+effect Exn (a: Type) (pre: ex_pre) (post: ex_post' a pre) =
+  EXN a (fun (p: ex_post a) -> pre /\ (forall (r: result a). post r ==> p r))
 
-let all_pre_h   (h:Type)           = h -> GTot Type0
-let all_post_h' (h:Type) (a:Type) (pre:Type)  = result a -> (_:h{pre}) -> GTot Type0
-let all_post_h  (h:Type) (a:Type)  = all_post_h' h a True
-let all_wp_h    (h:Type) (a:Type)  = all_post_h h a -> Tot (all_pre_h h)
+(** We include divergence in exceptions.
 
-unfold let all_ite_wp (heap:Type) (a:Type)
-                      (wp:all_wp_h heap a)
-                      (post:all_post_h heap a) (h0:heap) =
-    forall (k:all_post_h heap a).
-       (forall (x:result a) (h:heap).{:pattern (guard_free (k x h))} post x h ==> k x h)
-       ==> wp k h0
-unfold let all_return  (heap:Type) (a:Type) (x:a) (p:all_post_h heap a) = p (V x)
-unfold let all_bind_wp (heap:Type) (r1:range) (a:Type) (b:Type)
-                       (wp1:all_wp_h heap a)
-                       (wp2:(a -> GTot (all_wp_h heap b)))
-                       (p:all_post_h heap b) (h0:heap) : GTot Type0 =
-  wp1 (fun ra h1 -> (match ra with
-                  | V v     -> wp2 v p h1
-		  | E e     -> p (E e) h1
-		  | Err msg -> p (Err msg) h1)) h0
+    NOTE: BE WARNED, CODE IN THE [EXN] EFFECT IS ONLY CHECKED FOR
+    PARTIAL CORRECTNESS *)
+unfold
+let lift_div_exn (a: Type) (wp: pure_wp a) (p: ex_post a) = wp (fun a -> p (V a))
+sub_effect DIV ~> EXN { lift_wp = lift_div_exn }
 
-unfold let all_if_then_else (heap:Type) (a:Type) (p:Type)
-                             (wp_then:all_wp_h heap a) (wp_else:all_wp_h heap a)
-                             (post:all_post_h heap a) (h0:heap) =
-   l_ITE p
-       (wp_then post h0)
-       (wp_else post h0)
-unfold let all_stronger (heap:Type) (a:Type) (wp1:all_wp_h heap a)
-                        (wp2:all_wp_h heap a) =
-    (forall (p:all_post_h heap a) (h:heap). wp1 p h ==> wp2 p h)
+(** A variant of [Exn] with trivial pre- and postconditions *)
+effect Ex (a: Type) = Exn a True (fun v -> True)
 
-unfold let all_close_wp (heap:Type) (a:Type) (b:Type)
-                         (wp:(b -> GTot (all_wp_h heap a)))
-                         (p:all_post_h heap a) (h:heap) =
-    (forall (b:b). wp b p h)
-unfold let all_trivial (heap:Type) (a:Type) (wp:all_wp_h heap a) =
-    (forall (h0:heap). wp (fun r h1 -> True) h0)
+/// The [ALL_h] effect template for computations that may diverge,
+/// raise exceptions or fatal errors, and uses a generic state.
+///
+/// Note, this effect is poorly named, particularly as F* has since
+/// gained many more user-defined effect. We no longer have an effect
+/// that includes all others.
+///
+/// We might rename this in the future to something like [StExnDiv_h].
+///
+/// We layer state on top of exceptions, meaning that raising an
+/// exception does not discard the state.
+///
+/// As with [STATE_h], [ALL_h] is not a computation type, though its
+/// instantiation with a specific type of [heap] (in FStar.All) is.
 
+(** [all_pre_h] is a predicate on the initial state *)
+let all_pre_h (h: Type) = h -> GTot Type0
+
+(** Postconditions relate [result]s to final [heap]s refined by a precondition *)
+let all_post_h' (h a pre: Type) = result a -> _: h{pre} -> GTot Type0
+
+(** A variant of [all_post_h'] without the precondition refinement *)
+let all_post_h (h a: Type) = all_post_h' h a True
+
+(** WP predicate transformers for the [All_h] effect template *)
+let all_wp_h (h a: Type) = all_post_h h a -> Tot (all_pre_h h)
+
+(** Returning a value [x] normally promotes it to the [V x] result
+    without touching the [heap] *)
+unfold
+let all_return (heap a: Type) (x: a) (p: all_post_h heap a) = p (V x)
+
+(** Sequential composition for [ALL_h] is like [EXN]: case analysis of
+    the exceptional result before "running" the continuation *)
+unfold
+let all_bind_wp
+      (heap: Type)
+      (r1: range)
+      (a b: Type)
+      (wp1: all_wp_h heap a)
+      (wp2: (a -> GTot (all_wp_h heap b)))
+      (p: all_post_h heap b)
+      (h0: heap)
+    : GTot Type0 =
+  wp1 (fun ra h1 ->
+        (match ra with
+          | V v -> wp2 v p h1
+          | E e -> p (E e) h1
+          | Err msg -> p (Err msg) h1))
+    h0
+
+(** Case analysis in [ALL_h] *)
+unfold
+let all_if_then_else
+      (heap a p: Type)
+      (wp_then wp_else: all_wp_h heap a)
+      (post: all_post_h heap a)
+      (h0: heap)
+     = l_ITE p (wp_then post h0) (wp_else post h0)
+
+(** Naming postcondition for better sharing in [ALL_h] *)
+unfold
+let all_ite_wp (heap a: Type) (wp: all_wp_h heap a) (post: all_post_h heap a) (h0: heap) =
+  forall (k: all_post_h heap a).
+    (forall (x: result a) (h: heap). {:pattern (guard_free (k x h))} post x h ==> k x h) ==> wp k h0
+
+(** Subsumption in [ALL_h] *)
+unfold
+let all_stronger (heap a: Type) (wp1 wp2: all_wp_h heap a) =
+  (forall (p: all_post_h heap a) (h: heap). wp1 p h ==> wp2 p h)
+
+(** Closing a binder in the scope of an [ALL_h] wp *)
+unfold
+let all_close_wp
+      (heap a b: Type)
+      (wp: (b -> GTot (all_wp_h heap a)))
+      (p: all_post_h heap a)
+      (h: heap)
+     = (forall (b: b). wp b p h)
+
+(** Applying an [ALL_h] wp to a trivial postcondition *)
+unfold
+let all_trivial (heap a: Type) (wp: all_wp_h heap a) = (forall (h0: heap). wp (fun r h1 -> True) h0)
+
+(** Introducing the [ALL_h] effect template *)
 new_effect {
-  ALL_h (heap:Type) : a:Type -> wp:all_wp_h heap a -> Effect
+  ALL_h (heap: Type) : a: Type -> wp: all_wp_h heap a -> Effect
   with
-    return_wp    = all_return       heap
-  ; bind_wp      = all_bind_wp      heap
+    return_wp = all_return heap
+  ; bind_wp = all_bind_wp heap
   ; if_then_else = all_if_then_else heap
-  ; ite_wp       = all_ite_wp       heap
-  ; stronger     = all_stronger     heap
-  ; close_wp     = all_close_wp     heap
-  ; trivial      = all_trivial      heap
+  ; ite_wp = all_ite_wp heap
+  ; stronger = all_stronger heap
+  ; close_wp = all_close_wp heap
+  ; trivial = all_trivial heap
 }
 
-(* An SMT-pattern to control unfolding inductives;
-   In a proof, you can say `allow_inversion (option a)`
-   to allow the SMT solver. cf. allow_inversion below
- *)
-val inversion (a:Type) : Type0
+(**
+ Controlling inversions of inductive type
 
-val allow_inversion (a:Type)
-  : Pure unit (requires True) (ensures (fun x -> inversion a))
+ Given a value of an inductive type [v:t], where [t = A | B], the SMT
+ solver can only prove that [v=A \/ v=B] by _inverting_ [t]. This
+ inversion is controlled by the [ifuel] setting, which usually limits
+ the recursion depth of the number of such inversions that the solver
+ can perform.
 
-//allowing inverting option without having to globally increase the fuel just for this
-val invertOption : a:Type -> Lemma
-  (requires True)
-  (ensures (forall (x:option a). None? x \/ Some? x))
-  [SMTPat (option a)]
+ The [inversion] predicate below is a way to circumvent the
+ [ifuel]-based restrictions on inversion depth. In particular, if the
+ [inversion t] is available in the SMT solver's context, it is free to
+ invert [t] infinitely, regardless of the [ifuel] setting.
 
-type either 'a 'b =
-  | Inl : v:'a -> either 'a 'b
-  | Inr : v:'b -> either 'a 'b
+ Be careful using this, since it explicitly subverts the [ifuel]
+ setting. If used unwisely, this can lead to very poor SMT solver
+ performance.  *)
+val inversion (a: Type) : Type0
 
-let dfst (#a:Type) (#b:a -> GTot Type) (t:dtuple2 a b) : a = Mkdtuple2?._1 t
+(** To introduce [inversion t] in the SMT solver's context, call
+    [allow_inverson t]. *)
+val allow_inversion (a: Type) : Pure unit (requires True) (ensures (fun x -> inversion a))
 
-let dsnd (#a:Type) (#b:a -> GTot Type) (t:dtuple2 a b) : b (Mkdtuple2?._1 t) =
-  Mkdtuple2?._2 t
+(** Since the [option] type is so common, we always allow inverting
+    options, regardless of [ifuel] *)
+val invertOption (a: Type)
+    : Lemma (requires True) (ensures (forall (x: option a). None? x \/ Some? x)) [SMTPat (option a)]
 
-(* Concrete syntax (x:a & y:b x & c x y) *)
-unopteq type dtuple3 (a:Type)
-             (b:(a -> GTot Type))
-             (c:(x:a -> b x -> GTot Type)) =
-  | Mkdtuple3:_1:a
-             -> _2:b _1
-             -> _3:c _1 _2
-             -> dtuple3 a b c
+(** Values of type [a] or type [b] *)
+type either a b =
+  | Inl : v: a -> either a b
+  | Inr : v: b -> either a b
 
-(* Concrete syntax (x:a & y:b x & z:c x y & d x y z) *)
-unopteq type dtuple4 (a:Type)
-             (b:(x:a -> GTot Type))
-             (c:(x:a -> b x -> GTot Type))
-             (d:(x:a -> y:b x -> z:c x y -> GTot Type)) =
- | Mkdtuple4:_1:a
-           -> _2:b _1
-           -> _3:c _1 _2
-           -> _4:d _1 _2 _3
-           -> dtuple4 a b c d
+(** Projections for the components of a dependent pair *)
+let dfst (#a: Type) (#b: a -> GTot Type) (t: dtuple2 a b)
+    : Tot a
+  = Mkdtuple2?._1 t
 
-val ignore (#a:Type) (x:a) :Tot unit
+let dsnd (#a: Type) (#b: a -> GTot Type) (t: dtuple2 a b)
+    : Tot (b  (Mkdtuple2?._1 t))
+  = Mkdtuple2?._2 t
 
-val false_elim (#a:Type) (u:unit{false}) : Tot a
+(** Dependent triples, with sugar [x:a & y:b x & c x y] *)
+unopteq
+type dtuple3 (a: Type) (b: (a -> GTot Type)) (c: (x: a -> b x -> GTot Type)) =
+  | Mkdtuple3 : _1: a -> _2: b _1 -> _3: c _1 _2 -> dtuple3 a b c
 
+(** Dependent quadruples, with sugar [x:a & y:b x & z:c x y & d x y z] *)
+unopteq
+type dtuple4
+  (a: Type) (b: (x: a -> GTot Type)) (c: (x: a -> b x -> GTot Type))
+  (d: (x: a -> y: b x -> z: c x y -> GTot Type))
+  = | Mkdtuple4 : _1: a -> _2: b _1 -> _3: c _1 _2 -> _4: d _1 _2 _3 -> dtuple4 a b c d
 
-(* These are the supported attributes for top-level declarations. Syntax
- * example:
- *   [@ Gc ] type list a = | Nil | Cons of a * list a
- * or:
- *   [@ CInline ] let f x = UInt32.(x +%^ 1)
- *
- * Please add new attributes to this list along with a comment! Attributes are
- * desugared but not type-checked; using the constructors of a data type
- * guarantees a minimal amount of typo-checking.
- * *)
+(** Explicitly discarding a value *)
+val ignore (#a: Type) (x: a) : Tot unit
+
+(** In a context where [false] is provable, you can prove that any
+    type [a] is inhabited.
+
+    There are many proofs of this fact in F*. Here, in the implementation, we build an
+    infinitely looping function, since the termination check succeeds
+    in a [False] context. *)
+val false_elim (#a: Type) (u: unit{False}) : Tot a
+
+/// Attributes:
+///
+/// An attribute is any F* term.
+///
+/// Attributes are desugared and checked for being well-scoped. But,
+/// they are not type-checked.
+///
+/// It is associated with a definition using the [[@attribute]]
+/// notation, just preceding the definition.
+
+(** We collect several internal ocaml attributes into a single
+    inductive type.
+
+    This may be unnecessary. In the future, we are likely to flatten
+    this definition into several definitions of abstract top-level
+    names.
+
+    An example:
+
+     {[
+        [@ CInline ] let f x = UInt32.(x +%^ 1)
+      ]}
+
+    is extracted to C by KReMLin to a C definition tagged with the
+    [inline] qualifier. *)
 type __internal_ocaml_attributes =
   | PpxDerivingShow
-    (* Generate [@@ deriving show ] on the resulting OCaml type *)
-  | PpxDerivingShowConstant of string
-    (* Similar, but for constant printers. *)
-  | PpxDerivingYoJson
-    (* Generate [@@ deriving yojson ] on the resulting OCaml type *)
-  | CInline
-    (* KreMLin-only: generates a C "inline" attribute on the resulting
+  | PpxDerivingShowConstant of string (* Generate [@@ deriving show ] on the resulting OCaml type *)
+  | PpxDerivingYoJson (* Similar, but for constant printers. *)
+  | CInline (* Generate [@@ deriving yojson ] on the resulting OCaml type *)
+  (* KreMLin-only: generates a C "inline" attribute on the resulting
      * function declaration. *)
   | Substitute
-    (* KreMLin-only: forces KreMLin to inline the function at call-site; this is
+  (* KreMLin-only: forces KreMLin to inline the function at call-site; this is
      * deprecated and the recommended way is now to use F*'s
      * [inline_for_extraction], which now also works for stateful functions. *)
   | Gc
-    (* KreMLin-only: instructs KreMLin to heap-allocate any value of this
+  (* KreMLin-only: instructs KreMLin to heap-allocate any value of this
      * data-type; this requires running with a conservative GC as the
      * allocations are not freed. *)
   | Comment of string
-    (* KreMLin-only: attach a comment to the declaration. Note that using F*-doc
+  (* KreMLin-only: attach a comment to the declaration. Note that using F*-doc
      * syntax automatically fills in this attribute. *)
   | CPrologue of string
-    (* KreMLin-only: verbatim C code to be prepended to the declaration.
+  (* KreMLin-only: verbatim C code to be prepended to the declaration.
      * Multiple attributes are valid and accumulate, separated by newlines. *)
   | CEpilogue of string
-    (* Ibid. *)
-  | CConst of string
-    (* KreMLin-only: indicates that the parameter with that name is to be marked
+  | CConst of string (* Ibid. *)
+  (* KreMLin-only: indicates that the parameter with that name is to be marked
      * as C const.  This will be checked by the C compiler, not by KreMLin or F*.
      *
      * This is deprecated and doesn't work as intended. Use
      * LowStar.ConstBuffer.fst instead! *)
   | CCConv of string
-    (* A calling convention for C, one of stdcall, cdecl, fastcall *)
-  | CAbstractStruct
-    (* KreMLin-only: for types that compile to struct types (records and
+  | CAbstractStruct (* A calling convention for C, one of stdcall, cdecl, fastcall *)
+  (* KreMLin-only: for types that compile to struct types (records and
      * inductives), indicate that the header file should only contain a forward
      * declaration, which in turn forces the client to only ever use this type
      * through a pointer. *)
   | CIfDef
-    (* KreMLin-only: on a given `val foo`, compile if foo with #ifdef. *)
-  | CMacro
-    (* KreMLin-only: for a top-level `let v = e`, compile as a macro *)
+  | CMacro (* KreMLin-only: on a given `val foo`, compile if foo with #ifdef. *)
+(* KreMLin-only: for a top-level `let v = e`, compile as a macro *)
 
-(* Some supported attributes encoded using functions. *)
-
+(** The [inline_let] attribute on a local let-binding, instructs the
+    extraction pipeline to inline the definition. This may be both to
+    avoid generating unnecessary intermediate variables, and also to
+    enable further partial evaluation. Note, use this with care, since
+    inlining all lets can lead to an exponential blowup in code
+    size. *)
 val inline_let : unit
 
+(** The [rename_let] attribute support a form of metaprogramming for
+    the names of let-bound variables used in extracted code.
+
+    This is useful, particularly in conjunction with partial
+    evaluation, to ensure that names reflect their usage context.
+
+    See examples/micro-benchmarks/Renaming*.fst *)
 val rename_let (new_name: string) : Tot unit
 
-val plugin (x:int) : Tot unit
+(** The [plugin] attribute is used in conjunction with native
+    compilation of F* components, accelerating their reduction
+    relative to the default strategy of just interpreting them.
 
+    See examples/native_tactics for several examples. *)
+val plugin (x: int) : Tot unit
 
-(* An attribute to mark things that the typechecker should *first*
- * elaborate and typecheck, but unfold before verification. *)
+(** An attribute to mark things that the typechecker should *first*
+    elaborate and typecheck, but unfold before verification. *)
 val tcnorm : unit
 
-(*
- * we now erase all pure and ghost functions with unit return type to unit
- * this creates a small issue with abstract types. consider a module that
- * defines an abstract type t whose (internal) definition is unit and it also
- * defines a function f: int -> t.
- * with this new scheme, f would be erased to be just () inside the module
- * while the client calls to f would not, since t is abstract.
- * to get around this, when extracting interfaces, if we encounter an abstract type,
- * we will tag it with this attribute, so that extraction can treat it specially.
- *)
+(** We erase all ghost functions and unit-returning pure functions to
+    [()] at extraction. This creates a small issue with abstract
+    types. Consider a module that defines an abstract type [t] whose
+    (internal) definition is [unit] and also defines [f: int -> t]. [f]
+    would be erased to be just [()] inside the module, while the
+    client calls to [f] would not, since [t] is abstract. To get
+    around this, when extracting interfaces, if we encounter an
+    abstract type, we tag it with this attribute, so that
+    extraction can treat it specially.
+
+    Note, since the use of cross-module inlining (the [--cmi] option),
+    this attribute is no longer necessary. We retain it for legacy,
+    but will remove it in the future. *)
 val must_erase_for_extraction : unit
 
+(** This attribute is used with the Dijkstra Monads for Free
+    construction to track position information in generated VCs *)
 val dm4f_bind_range : unit
 
 (** When attached a top-level definition, the typechecker will succeed
- * if and only if checking the definition results in an error. The
- * error number list is actually OPTIONAL. If present, it will be
- * checked that the definition raises exactly those errors in the
- * specified multiplicity, but order does not matter. *)
-val expect_failure (errs : list int) : Tot unit
+    if and only if checking the definition results in an error. The
+    error number list is actually OPTIONAL. If present, it will be
+    checked that the definition raises exactly those errors in the
+    specified multiplicity, but order does not matter. *)
+val expect_failure (errs: list int) : Tot unit
 
-(** When --lax is present, we the previous attribute since some definitions
- * only fail when verification is turned on. With this attribute, one can ensure
- * that a definition fails while lax-checking too. Same semantics as above,
- * but lax mode will be turned on for the definition.
- *)
-val expect_lax_failure (errs : list int) : Tot unit
+(** When --lax is present, with the previous attribute since some
+  definitions only fail when verification is turned on. With this
+  attribute, one can ensure that a definition fails while lax-checking
+  too. Same semantics as above, but lax mode will be turned on for the
+  definition.  *)
+val expect_lax_failure (errs: list int) : Tot unit
 
 (** Print the time it took to typecheck a top-level definition *)
 val tcdecltime : unit
 
-(**
- * **THIS ATTRIBUTE IS AN ESCAPE HATCH AND CAN BREAK SOUNDNESS**
- * **USE WITH CARE**
- * The positivity check for inductive types stops at abstraction
- * boundaries. This results in spurious errors about positivity,
- * e.g., when defining types like `type t = ref (option t)`
- * By adding this attribute to a declaration of a top-level name
- * positivity checks on applications of that name are admitted.
- * See, for instance, FStar.Monotonic.Heap.mref
- * We plan to decorate binders of abstract types with polarities
- * to allow us to check positivity across abstraction boundaries
- * and will eventually remove this attribute.
- *)
+(** **THIS ATTRIBUTE IS AN ESCAPE HATCH AND CAN BREAK SOUNDNESS**
+
+    **USE WITH CARE**
+
+    The positivity check for inductive types stops at abstraction
+    boundaries. This results in spurious errors about positivity,
+    e.g., when defining types like `type t = ref (option t)` By adding
+    this attribute to a declaration of a top-level name positivity
+    checks on applications of that name are admitted.  See, for
+    instance, FStar.Monotonic.Heap.mref We plan to decorate binders of
+    abstract types with polarities to allow us to check positivity
+    across abstraction boundaries and will eventually remove this
+    attribute.  *)
 val assume_strictly_positive : unit
 
-(**
- * This attribute is to be used as a hint for the unifier.
- * A function-typed symbol `t` marked with this attribute
- * will be treated as being injective in all its arguments
- * by the unifier.
- * That is, given a problem `t a1..an =?= t b1..bn`
- * the unifier will solve it by proving `ai =?= bi` for
- * all `i`, without trying to unfold the definition of `t`.
- **)
+(** This attribute is to be used as a hint for the unifier.  A
+    function-typed symbol `t` marked with this attribute will be treated
+    as being injective in all its arguments by the unifier.  That is,
+    given a problem `t a1..an =?= t b1..bn` the unifier will solve it by
+    proving `ai =?= bi` for all `i`, without trying to unfold the
+    definition of `t`. *)
 val unifier_hint_injective : unit
 
 (**
- * This attribute is used to control the evaluation order
- * and unfolding strategy for certain definitions.
- *
- * In particular, given
- *    [@(strict_on_arguments [1;2])]
- *    let f x0 (x1:list x0) (x1:option x0) = e
- *
- * An application `f e0 e1 e2` is reduced by the normalizer by:
- *   1. evaluating e0 ~>* v0, e1 ~>* v1, e2 ~>* v2
- *
- *   2 a.
- *      If, according to the positional arguments [1;2],
- *      if v1 and v2 have constant head symbols
- *             (e.g., v1 = Cons _ _ _, and v2 = None _)
- *      then `f` is unfolded to `e` and reduced as
- *        e[v0/x0][v1/x1][v2/x2]
- *
- *   2 b.
- *
- *     Otherwise, `f` is not unfolded and the term is `f e0 e1 e2`
- *     reduces to `f v0 v1 v2`.
- *
- *)
-val strict_on_arguments (x:list int) : Tot unit
+ This attribute is used to control the evaluation order
+ and unfolding strategy for certain definitions.
+
+  In particular, given
+     {[
+        [@(strict_on_arguments [1;2])]
+        let f x0 (x1:list x0) (x1:option x0) = e
+     ]}
+
+ An application [f e0 e1 e2] is reduced by the normalizer by:
+
+     1. evaluating [e0 ~>* v0, e1 ~>* v1, e2 ~>* v2]
+
+     2 a.
+        If, according to the positional arguments [1;2],
+        if v1 and v2 have constant head symbols
+              (e.g., v1 = Cons _ _ _, and v2 = None _)
+       then [f] is unfolded to [e] and reduced as
+         {[e[v0/x0][v1/x1][v2/x2]]}
+
+     2 b.
+
+      Otherwise, [f] is not unfolded and the term is [f e0 e1 e2]
+      reduces to [f v0 v1 v2]. *)
+val strict_on_arguments (x: list int) : Tot unit
 
 (**
  * An attribute to tag a tactic designated to solve any
@@ -447,68 +625,135 @@ val strict_on_arguments (x:list int) : Tot unit
  **)
 val resolve_implicits : unit
 
-(*
- * This attribute can be added to an inductive type definition,
- * indicating that it should be erased on extraction to `unit`.
- *
- * However, any pattern matching on the inductive type results
- * in a `Ghost` effect, ensuring that computationally relevant
- * code cannot rely on the values of the erasable type.
- *
- * See examples/micro-benchmarks/Erasable.fst, for examples.
- * Also see https://github.com/FStarLang/FStar/issues/1844
- *)
+(** This attribute can be added to an inductive type definition,
+    indicating that it should be erased on extraction to `unit`.
+
+    However, any pattern matching on the inductive type results
+    in a `Ghost` effect, ensuring that computationally relevant
+    code cannot rely on the values of the erasable type.
+
+    See examples/micro-benchmarks/Erasable.fst, for examples.  Also
+    see https://github.com/FStarLang/FStar/issues/1844 *)
 val erasable : unit
 
-(*********************************************************************************)
-(* Marking terms for normalization *)
-(*********************************************************************************)
-val normalize_term (#a:Type) (x:a) : Tot a
-val normalize (a:Type0) : Tot Type0
+///  Controlling normalization
 
+(** In any invocation of the F* normalizer, every occurrence of
+    [normalize_term e] is reduced to the full normal for of [e]. *)
+val normalize_term (#a: Type) (x: a) : Tot a
+
+(** In any invocation of the F* normalizer, every occurrence of
+    [normalize e] is reduced to the full normal for of [e]. *)
+val normalize (a: Type0) : Type0
+
+(** Value of [norm_step] are used to enable specific normalization
+    steps, controlling how the normalizer reduces terms. *)
 val norm_step : Type0
 
+(** Logical simplification, e.g., [P /\ True ~> P] *)
 val simplify : norm_step
-val weak     : norm_step
-val hnf      : norm_step
-val primops  : norm_step
-val delta    : norm_step
-val zeta     : norm_step
-val iota     : norm_step
-val nbe      : norm_step  // use NBE instead of the normalizer
-val reify_   : norm_step
-val delta_only  (s : list string) : Tot norm_step  // each string is a fully qualified name like `A.M.f`
-val delta_fully (s : list string) : Tot norm_step  // idem
-val delta_attr  (s : list string) : Tot norm_step
 
-// Normalization marker
-val norm (s:list norm_step) (#a:Type) (x:a) : Tot a
+(** Weak reduction: Do not reduce under binders *)
+val weak : norm_step
 
-val assert_norm : p:Type -> Pure unit (requires (normalize p)) (ensures (fun _ -> p))
+(** Head normal form *)
+val hnf : norm_step
 
+(** Reduce primitive operators, e.g., [1 + 1 ~> 2] *)
+val primops : norm_step
+
+(** Unfold all non-recursive definitions *)
+val delta : norm_step
+
+(** Unroll recursive calls *)
+val zeta : norm_step
+
+(** Reduce case analysis (i.e., match) *)
+val iota : norm_step
+
+(** Use normalization-by-evaluation, instead of interpretation (experimental) *)
+val nbe : norm_step
+
+(** Reify effectful definitions into their representations *)
+val reify_ : norm_step
+
+(** Unlike [delta], unfold definitions for only the names in the given
+    list. Each string is a fully qualified name like [A.M.f] *)
+val delta_only (s: list string) : Tot norm_step
+
+(** Unfold definitions for only the names in the given list, but
+    unfold each definition encountered after unfolding as well.
+
+    For example, given
+
+      {[
+        let f0 = 0
+        let f1 = f0 + 1
+      ]}
+
+    [norm [delta_only [`%f1]] f1] will reduce to [f0 + 1].
+    [norm [delta_fully [`%f1]] f1] will reduce to [0 + 1].
+
+    Each string is a fully qualified name like [A.M.f], typically
+    constructed using a quotation, as in the example above. *)
+val delta_fully (s: list string) : Tot norm_step
+
+(** Rather than mention a symbol to unfold by name, it can be
+    convenient to tag a collection of related symbols with a common
+    attribute and then to ask the normalizer to reduce them all.
+
+    For example, given:
+
+      {[
+        irreducible let my_attr = ()
+
+        [@my_attr]
+        let f0 = 0
+
+        [@my_attr]
+        let f1 = f0 + 1
+      ]}
+
+   {[norm [delta_attr [`%my_attr]] f1]}
+   
+   will reduce to [0 + 1].
+
+  *)
+val delta_attr (s: list string) : Tot norm_step
+
+(** [norm s e] requests normalization of [e] with the reduction steps
+    [s]. *)
+val norm (s: list norm_step) (#a: Type) (x: a) : Tot a
+
+(** [assert_norm p] reduces [p] as much as possible and then asks the
+    SMT solver to prove the reduct, concluding [p] *)
+val assert_norm (p: Type) : Pure unit (requires (normalize p)) (ensures (fun _ -> p))
+
+(** Sometimes it is convenient to introduce an equation between a term
+    and its normal form in the context. *)
 val normalize_term_spec (#a: Type) (x: a) : Lemma (normalize_term #a x == x)
+
+(** Like [normalize_term_spec], but specialized to [Type0] *)
 val normalize_spec (a: Type0) : Lemma (normalize a == a)
+
+(** Like [normalize_term_spec], but with specific normalization steps *)
 val norm_spec (s: list norm_step) (#a: Type) (x: a) : Lemma (norm s #a x == x)
 
-(*
- * Use the following to expose an `opaque_to_smt` definition to the solver
- *   as: `reveal_opaque (`%defn) defn
- *)
-let reveal_opaque (s:string) = norm_spec [delta_only [s]]
+(** Use the following to expose an ["opaque_to_smt"] definition to the
+    solver as: [reveal_opaque (`%defn) defn] *)
+let reveal_opaque (s: string) = norm_spec [delta_only [s]]
 
-(*
- * Pure and ghost inner let bindings are now always inlined during the wp computation, if:
- * the return type is not unit and the head symbol is not marked irreducible.
- * To circumvent this behavior, singleton can be used.
- * See the example usage in ulib/FStar.Algebra.Monoid.fst.
- *)
-val singleton (#a:Type) (x:a) : Tot (y:a{y == x})
+(** Pure and ghost inner let bindings are now always inlined during
+    the wp computation, if: the return type is not unit and the head
+    symbol is not marked irreducible.
 
+    To circumvent this behavior, singleton can be used.
+    See the example usage in ulib/FStar.Algebra.Monoid.fst. *)
+val singleton (#a: Type) (x: a) : Tot (y: a{y == x})
 
-(*
- * `with_type t e` is just an identity function, but it receives special treatment
- *  in the SMT encoding, where in addition to being an identity function, we have
- *  an SMT axiom:
- *  `forall t e.{:pattern (with_type t e)} has_type (with_type t e) t`
- *)
-val with_type (#t:Type) (e:t) : Tot t
+(** [with_type t e] is just an identity function, but it receives
+    special treatment in the SMT encoding, where in addition to being
+    an identity function, we have an SMT axiom:
+    [forall t e.{:pattern (with_type t e)} has_type (with_type t e) t] *)
+val with_type (#t: Type) (e: t) : Tot t
+
